Subroutine lemma proof

LeanScratch/Computation/RegMachine/Subroutine.lean
@@ -1,229 +1,38 @@
 import LeanScratch.Computation.RegMachine
 import LeanScratch.Computation.RegMachine.UpdateImage
+import LeanScratch.Computation.RegMachine.Subroutine.Ins
+import LeanScratch.Computation.RegMachine.Subroutine.Reg
 
 namespace Comp
 
-variable {Ins InsB} [Fintype2 Ins] [Fintype2 InsB]
-
-def subroutine.insMapper
-    {r : RegTree}
-    (inM : RegMachine r Ins)
-    (imapper : Ins → InsB)
-    (hltStepper : InsB)
-    (x : Ins) : RegMachine.Ins r InsB :=
-  match inM x with
-  | .inc r next =>
-    let next := match inM next with
-      | .hlt => hltStepper
-      | _    => imapper next
-    .inc r next
-  | .dec r nz z =>
-    let nz := match inM nz with
-      | .hlt => hltStepper
-      | _    => imapper nz
-    let z  := match inM z with
-      | .hlt => hltStepper
-      | _    => imapper z
-    .dec r nz z
-  | .hlt => .hlt -- This case should be handled differently maybe
-
-def subroutine.regMapper
+variable {InsA InsB} [Fintype2 InsA] [Fintype2 InsB]
+def subroutine
     {r t : RegTree}
-    (inM : RegMachine r Ins)
-    (rmapper : r.toIdx → t.toIdx)
-    : RegMachine t Ins :=
-  (match inM · with
-  | .inc reg ins => .inc (rmapper reg) ins
-  | .dec reg nz z => .dec (rmapper reg) nz z
-  | .hlt => .hlt)
-
-/- def subroutine -/
-/-     {r t : RegTree} -/
-/-     (inM : RegMachine r Ins) -/
-/-     (rmapper : r.toIdx → t.toIdx) -/
-/-     (imapper : Ins → InsB) -/
-/-     (hltStepper : InsB) -/
-/-     (x : Ins) -/
-/-     : RegMachine.Ins t InsB := -/
-/-   subroutine.regMapper (subroutine.regMapper inM rmapper) _ _ x -/
-
-theorem RegMachine.step.none_hlt [Fintype2 L] {inM : RegMachine r L}
-    (h : RegMachine.Config.step inM ⟨view, s⟩ = none)
-    : inM s = .hlt :=
-  match heq : inM s with
-  | .hlt => rfl
-  | .inc _ _ | .dec _ _ _ => by
-    simp only [Config.step, heq] at h
-    <;> split at h
-    <;> exact Option.noConfusion h
-
-theorem subroutine.regMapper.singleForward
-    {r t : RegTree}
-    {inM : RegMachine r Ins}
-    {map : r.toIdx → t.toIdx}
-    {inS outS defS}
-    (hRInj : Function.Injective map)
-    (hBStep : RegMachine.Config.step inM ⟨inS, s1⟩ = some ⟨outS, s2⟩)
-    : RegMachine.Config.step (subroutine.regMapper inM map)
-      ⟨updateImage map inS defS, s1⟩ =
-      some ⟨updateImage map outS defS, s2⟩ := by
-  dsimp [RegMachine.Config.step, regMapper] at *
-  split at hBStep
-  <;> rename_i hMEq
-  · rcases hBStep with ⟨rfl, rfl⟩
-    simp only [hMEq, Option.some.injEq, RegMachine.Config.mk.injEq, and_true]
-    exact updateImage.inc_slide hRInj
-  · split at hBStep
-    <;> rcases hBStep with ⟨rfl, rfl⟩
-    <;> rename_i hDecEq
-    <;> simp only [hMEq]
-    · rw [updateImage.dec_slide hRInj, hDecEq]
-      rfl
-    · rename_i r _ _
-      rw [RegMachine.dec_none_iff_lookup_z] at hDecEq
-      have this : RegMachine.dec _ (updateImage map inS defS) = none :=
-        RegMachine.dec_none_iff_lookup_z.mpr
-        $ Eq.trans (updateImage.lookup hRInj) hDecEq
-      simp [this]
-  · exact Option.noConfusion hBStep
-
--- TODO: Split this into a simpler lemma where I just do it on a single step
---       and a driver lemma that does the whole computation.
-theorem subroutine.insMapper.forward
-    {r : RegTree}
-    {prog : RegMachine r InsB}
-    {inM  : RegMachine r Ins}
-
-    {imapper iInitStore iEndStore}
-
-    -- the following theorems should all be solvable with large simps
-    (hIsSub : prog ∘ imapper = insMapper inM imapper hltStepper)
-
-    (hInTW : inM.TW ⟨iInitStore, startS⟩ ⟨iEndStore, endS⟩)
-    (hStartNotHlt : inM startS ≠ .hlt)
-
-    : prog.StepsTo ⟨iInitStore, imapper startS⟩
-                   ⟨iEndStore, hltStepper⟩ := by
-  rcases hInTW with ⟨w, term, v⟩
-  exists w
-  induction w generalizing startS iInitStore
-  · obtain ⟨rfl, rfl⟩ := (RegMachine.Config.mk.injEq _ _ _ _).mp $ (Option.some.injEq _ _).mp term
-    exact (hStartNotHlt $ RegMachine.step.none_hlt v).elim
-  case succ n ih =>
-    -- Unfold what information we get about the termination
-    obtain ⟨⟨imStore, imState⟩, stepper, p⟩ := Option.bind_eq_some.mp term; clear term
-
-    apply Option.bind_eq_some.mpr
-
-    -- Open the step defn
-    simp only [Function.funext_iff, Function.comp_apply] at hIsSub
-    dsimp [RegMachine.Config.step]
-    rw [hIsSub]; clear hIsSub
-
-    dsimp [insMapper]
-    cases heq : inM startS
-    <;> dsimp
-    <;> simp only [RegMachine.Config.step, heq, Option.some.injEq, RegMachine.Config.mk.injEq] at stepper
-    <;> clear heq
-    case inc reg nextins =>
-      rcases stepper with ⟨rfl, rfl⟩
-      by_cases hNextEq : inM nextins = .hlt
-      · exists ⟨RegMachine.inc reg iInitStore, hltStepper⟩
-        simp only [hNextEq, true_and]
-        obtain rfl : n = 0 := by
-          cases n
-          · rfl
-          · simp [RegMachine.Config.step_n, RegMachine.Config.step, hNextEq] at p
-        simp_all
-      · simp only [Option.some.injEq, exists_eq_left', hNextEq]
-        apply ih hNextEq
-        rw [←p]
-    case dec r nzdest zdest =>
-      split
-      <;> rename_i heq
-      <;> simp only [heq, Option.some.injEq, RegMachine.Config.mk.injEq] at stepper
-      <;> rcases stepper with ⟨rfl, rfl⟩
-      next x s =>
-        by_cases hNextEq : inM nzdest = .hlt
-        · exists ⟨s, hltStepper⟩
-          simp only [hNextEq, true_and]
-          obtain rfl : n = 0 := by
-            cases n
-            · rfl
-            · simp [RegMachine.Config.step_n, RegMachine.Config.step, hNextEq] at p
-          simp_all
-        · simp only [Option.some.injEq, exists_eq_left']
-          apply ih hNextEq
-          rw [←p]
-      next s =>
-        by_cases hNextEq : inM zdest = .hlt
-        · exists ⟨iInitStore, hltStepper⟩
-          obtain rfl : n = 0 := by
-            cases n
-            · rfl
-            · simp [RegMachine.Config.step_n, RegMachine.Config.step, hNextEq] at p
-          simp_all
-        · simp only [Option.some.injEq, exists_eq_left']
-          apply ih hNextEq p
+    : (RegMachine r InsA) → (r.toIdx → t.toIdx)
+    → (InsA → InsB) → InsB → InsA
+    → RegMachine.Ins t InsB :=
+  (subroutine.insMapper $ subroutine.regMapper · ·)
 
 theorem subroutine.forward
     {r t : RegTree}
     {prog : RegMachine t InsB}
 
-    {inM : RegMachine r Ins}
+    {inM : RegMachine r InsA}
     {rmapper : r.toIdx → t.toIdx}
-    {imapper : Ins → InsB}
+    {imapper : InsA → InsB}
 
     {iInitStore iEndStore outerStore}
 
     -- the following theorems should all be solvable with large simps
     (hIsSub : prog ∘ imapper = subroutine inM rmapper imapper hltStepper)
-
     (hRInj : Function.Injective rmapper)
-    (hIInj : Function.Injective imapper)
-
-    (hInTW : inM.TW ⟨iInitStore, startS⟩ ⟨iEndStore, endS⟩)
     (hStartNotHlt : inM startS ≠ .hlt)
 
-    : prog.StepsTo ⟨updateImage rmapper iInitStore outerStore, imapper startS⟩
-                   ⟨updateImage rmapper iEndStore  outerStore, hltStepper⟩ := by
-  rcases hInTW with ⟨w, term, v⟩
-  induction w generalizing startS iInitStore
-  · obtain ⟨rfl, rfl⟩ := (RegMachine.Config.mk.injEq _ _ _ _).mp $ (Option.some.injEq _ _).mp term
-    exact (hStartNotHlt $ RegMachine.step.none_hlt v).elim
-  case succ n ih =>
-    obtain ⟨⟨imStore, imState⟩, stepper, p⟩ := Option.bind_eq_some.mp term
-    clear term
+    (hInTW : inM.TW ⟨iInitStore, startS⟩ ⟨iEndStore, endS⟩)
 
-    exists n+1
-    simp only [RegMachine.Config.step_n]
-    apply Option.bind_eq_some.mpr
-    dsimp [RegMachine.Config.step, subroutine]
-    simp [Function.funext_iff] at hIsSub
-    rw [hIsSub]
-    dsimp [subroutine]
-    cases heq : inM startS
-    <;> (try exact (hStartNotHlt heq).elim)
-    <;> rename_i reg nextins
-    <;> by_cases hNextEq : inM nextins = .hlt
-    · clear ih
-      use ⟨RegMachine.inc (rmapper reg) (updateImage rmapper iInitStore outerStore), hltStepper⟩
-      simp [hNextEq]
-      simp only [RegMachine.Config.step, heq, Option.some.injEq, RegMachine.Config.mk.injEq] at stepper
-      rcases stepper with ⟨rfl, rfl⟩
-      obtain rfl : n = 0 := by
-        cases n
-        · rfl
-        · simp [RegMachine.Config.step_n, RegMachine.Config.step, hNextEq] at p
-      simp_all only [ne_eq, not_false_eq_true, RegMachine.Config.step_n.zero, Option.some.injEq,
-        RegMachine.Config.mk.injEq, and_true]
-      rcases p with ⟨rfl, rfl⟩
-      sorry
-      /- by_cases hInImage : ∃ v', v = rmapper v' -/
-      /- sorry -/
-      /- · have := hNeqStores _ hInImage -/
-      /-   sorry -/
-    · sorry
-    · sorry
-    · sorry
+    : prog.StepsTo ⟨updateImage rmapper iInitStore outerStore, imapper startS⟩
+                   ⟨updateImage rmapper iEndStore  outerStore, hltStepper⟩ :=
+  subroutine.insMapper.forward hIsSub (regMapper.neLift hStartNotHlt)
+    $ subroutine.regMapper.forward hRInj hInTW
+
 
