LeanScratch/Computation/RegMachine/Subroutine/Ins.lean
@@ -1,0 +1,95 @@
+import LeanScratch.Computation.RegMachine
+
+namespace Comp
+
+variable {InsA InsB} [Fintype2 InsA] [Fintype2 InsB]
+
+def subroutine.insMapper
+    {r : RegTree}
+    (inM : RegMachine r InsA)
+    (imapper : InsA → InsB)
+    (hltStepper : InsB)
+    (x : InsA) : RegMachine.Ins r InsB :=
+  match inM x with
+  | .inc r next =>
+    let next := match inM next with
+      | .hlt => hltStepper
+      | _    => imapper next
+    .inc r next
+  | .dec r nz z =>
+    let nz := match inM nz with
+      | .hlt => hltStepper
+      | _    => imapper nz
+    let z  := match inM z with
+      | .hlt => hltStepper
+      | _    => imapper z
+    .dec r nz z
+  | .hlt => .hlt -- This case should be handled differently maybe
+
+-- TODO: Split this into a simpler lemma where I just do it on a single step
+--       and a driver lemma that does the whole computation.
+theorem subroutine.insMapper.forward
+    {r : RegTree}
+    {prog : RegMachine r InsB}
+    {inM  : RegMachine r InsA}
+
+    {imapper iInitStore iEndStore}
+
+    -- the following theorems should all be solvable with large simps
+    (hIsSub : prog ∘ imapper = insMapper inM imapper hltStepper)
+    (hStartNotHlt : inM startS ≠ .hlt)
+
+    (hInTW : inM.TW ⟨iInitStore, startS⟩ ⟨iEndStore, endS⟩)
+
+    : prog.StepsTo ⟨iInitStore, imapper startS⟩
+                   ⟨iEndStore, hltStepper⟩ := by
+  rcases hInTW with ⟨w, term, v⟩
+  exists w
+  induction w generalizing startS iInitStore
+  · obtain ⟨rfl, rfl⟩ := (RegMachine.Config.mk.injEq _ _ _ _).mp $ (Option.some.injEq _ _).mp term
+    exact (hStartNotHlt $ RegMachine.Config.step.none_hlt v).elim
+  case succ n ih =>
+    -- Unfold what information we get about the termination
+    obtain ⟨⟨imStore, imState⟩, stepper, p⟩ := Option.bind_eq_some.mp term; clear term
+
+    apply Option.bind_eq_some.mpr
+
+    -- Open the step defn
+    simp only [Function.funext_iff, Function.comp_apply] at hIsSub
+    dsimp [RegMachine.Config.step]
+    rw [hIsSub]; clear hIsSub
+
+    dsimp [insMapper]
+    cases heq : inM startS
+    <;> dsimp
+    <;> simp only [RegMachine.Config.step, heq, Option.some.injEq, RegMachine.Config.mk.injEq] at stepper
+    <;> clear heq
+    on_goal 1 =>  rename_i reg nextins
+    on_goal 2 => (rename_i reg nzdest zdest; split <;> rename_i heq <;>
+      simp only [heq, Option.some.injEq, RegMachine.Config.mk.injEq] at stepper)
+
+    all_goals rcases stepper with ⟨rfl, rfl⟩
+
+    -- Split each case
+    on_goal 1 => by_cases hNextEq : inM nextins = .hlt
+    on_goal 3 => by_cases hNextEq : inM nzdest  = .hlt
+    on_goal 5 => by_cases hNextEq : inM zdest   = .hlt
+
+    -- Close negative goals
+    any_goals (simp only [Option.some.injEq, exists_eq_left']; exact ih hNextEq p)
+
+    -- Assign each store value
+    on_goal 1 => exists ⟨RegMachine.inc reg iInitStore, hltStepper⟩
+    on_goal 3 => exists ⟨iInitStore,                    hltStepper⟩
+    on_goal 2 => rename_i s;                 exists ⟨s, hltStepper⟩
+
+    -- Close all goals
+    all_goals {
+      simp only [hNextEq, true_and]
+      obtain rfl : n = 0 := by
+        cases n
+        · rfl
+        · simp [RegMachine.Config.step_n, RegMachine.Config.step, hNextEq] at p
+      simp_all
+    }
+
