LeanScratch/Computation/RegMachine/Subroutine/Reg.lean
@@ -1,0 +1,78 @@
+import LeanScratch.Computation.RegMachine
+import LeanScratch.Computation.RegMachine.UpdateImage
+
+namespace Comp
+
+variable {InsA InsB} [Fintype2 InsA] [Fintype2 InsB]
+
+def subroutine.regMapper
+    {r t : RegTree}
+    (inM : RegMachine r InsA)
+    (rmapper : r.toIdx → t.toIdx)
+    : RegMachine t InsA :=
+  (match inM · with
+  | .inc reg ins => .inc (rmapper reg) ins
+  | .dec reg nz z => .dec (rmapper reg) nz z
+  | .hlt => .hlt)
+
+def subroutine.regMapper.neLift
+    {r t : RegTree}
+    {inM : RegMachine r InsA}
+    {rmapper : r.toIdx → t.toIdx}
+    (h : inM s ≠ .hlt)
+    : regMapper inM rmapper s ≠ .hlt := by
+  dsimp [regMapper]
+  cases hEq : inM s <;> simp_all
+
+theorem subroutine.regMapper.singleForward
+    {r t : RegTree}
+    {inM : RegMachine r InsA}
+    {map : r.toIdx → t.toIdx}
+    {inS outS defS}
+    (hRInj : Function.Injective map)
+    (hBStep : RegMachine.Config.step inM ⟨inS, s1⟩ = some ⟨outS, s2⟩)
+    : RegMachine.Config.step (subroutine.regMapper inM map)
+      ⟨updateImage map inS defS, s1⟩ =
+      some ⟨updateImage map outS defS, s2⟩ := by
+  dsimp [RegMachine.Config.step, regMapper] at *
+  split at hBStep
+  <;> rename_i hMEq
+  · rcases hBStep with ⟨rfl, rfl⟩
+    simp only [hMEq, Option.some.injEq, RegMachine.Config.mk.injEq, and_true]
+    exact updateImage.inc_slide hRInj
+  · split at hBStep
+    <;> rcases hBStep with ⟨rfl, rfl⟩
+    <;> rename_i hDecEq
+    <;> simp only [hMEq]
+    · rw [updateImage.dec_slide hRInj, hDecEq]
+      rfl
+    · rename_i r _ _
+      rw [RegMachine.dec_none_iff_lookup_z] at hDecEq
+      have this : RegMachine.dec _ (updateImage map inS defS) = none :=
+        RegMachine.dec_none_iff_lookup_z.mpr
+        $ Eq.trans (updateImage.lookup hRInj) hDecEq
+      simp [this]
+  · exact Option.noConfusion hBStep
+
+theorem subroutine.regMapper.forward
+    {r t : RegTree}
+    {inM : RegMachine r InsA}
+    {map : r.toIdx → t.toIdx}
+    {inS outS defS}
+    (hRInj : Function.Injective map)
+    (hBStep : inM.TW ⟨inS, s1⟩ ⟨outS, s2⟩)
+    : (subroutine.regMapper inM map).TW
+        ⟨updateImage map inS defS, s1⟩
+        ⟨updateImage map outS defS, s2⟩ := by
+  rcases hBStep with ⟨n, p, hTerm⟩
+  exists n
+  induction n generalizing inS s1
+  · rcases p with ⟨rfl, rfl⟩
+    refine ⟨rfl, ?_⟩
+    dsimp [RegMachine.Config.step, regMapper]
+    rw [RegMachine.Config.step.none_hlt hTerm]
+  case succ ih =>
+    dsimp [RegMachine.Config.step_n] at *
+    have ⟨⟨imS, imI⟩, hSmall, hLong⟩ := Option.bind_eq_some.mp p; clear p
+    rw [regMapper.singleForward hRInj hSmall, Option.some_bind]
+    exact ih hLong
